Tests/Utils/Vector.lean
@@ -6,8 +6,10 @@ private def v6 : Vector Nat 6 := #v[1, 2, 3, 4, 5, 6]
 private def chunks {α : Type} {n m : Nat} (v : Vector (Vector α m) n) : List (List α) :=
   v.toList.map (·.toList)
 
-example : chunks (v6.toChunks 3 2) = [[1, 2], [3, 4], [5, 6]] := by native_decide
-example : chunks (v6.toChunks 1 6) = [[1, 2, 3, 4, 5, 6]] := by native_decide
-example : chunks (v6.toChunks 6 1) = [[1], [2], [3], [4], [5], [6]] := by native_decide
-example : chunks ((#v[] : Vector Nat 0).toChunks 0 4) = [] := by native_decide
-example : chunks ((#v[] : Vector Nat 0).toChunks 2 0) = [[], []] := by native_decide
+example : chunks (v6.toChunks 2) = [[1, 2], [3, 4], [5, 6]] := by native_decide
+example : chunks (v6.toChunks 6) = [[1, 2, 3, 4, 5, 6]] := by native_decide
+example : chunks (v6.toChunks 1) = [[1], [2], [3], [4], [5], [6]] := by native_decide
+-- The remainder is dropped.
+example : chunks (v6.toChunks 4) = [[1, 2, 3, 4]] := by native_decide
+example : chunks (v6.toChunks 7) = [] := by native_decide
+example : chunks ((#v[] : Vector Nat 0).toChunks 4) = [] := by native_decide
